compiler/core/EJson/EJsonRuntime.v
@@ -17,4 +17,5 @@ Require Export EJson.
 Require Export EJsonNorm.
 Require Export ForeignEJsonRuntime.
 Require Export EJsonOperators.
+Require Export EJsonGroupBy.
 Require Export EJsonRuntimeOperators.
