compiler/core/EJson/Operators/EJsonGroupBy.v
@@ -1,0 +1,80 @@
+(*
+ * Licensed under the Apache License, Version 2.0 (the "License");
+ * you may not use this file except in compliance with the License.
+ * You may obtain a copy of the License at
+ *
+ * http://www.apache.org/licenses/LICENSE-2.0
+ *
+ * Unless required by applicable law or agreed to in writing, software
+ * distributed under the License is distributed on an "AS IS" BASIS,
+ * WITHOUT WARRANTIES OR CONDITIONS OF ANY KIND, either express or implied.
+ * See the License for the specific language governing permissions and
+ * limitations under the License.
+ *)
+
+Require Import List.
+Require Import String.
+Require Import Utils.
+Require Import Iterators.
+Require Import Bindings.
+Require Import ForeignEJson.
+Require Import EJson.
+
+Section EJsonGroupBy.
+  Context {fejson:foreign_ejson}.
+  Import ListNotations.
+
+  (* Alternate semantics, using nested loop -- closer to NRC encoding of group by *)
+
+  (* Note: split the proof in two:
+       - define a nested-loop based group-by
+       - prove that nested-loop based group-by is equivalent to Louis' group-by
+       - prove that nested NRC group-by is same as nested-loop group-by
+   *)
+
+  (* key eval. there are really two forms. one form is symmetric,
+     while the other works when the key computation has been split in two
+     phases. which one to use depends on the group-by algorithm *)
+
+  Definition ejson_key_is_eq_r (eval_key: ejson -> option ejson) (d1 d2:ejson) : option bool :=
+    olift2 (fun x y => if ejson_eq_dec x y then Some true else Some false)
+           (eval_key d1)
+           (Some d2).
+
+  Definition ejson_group_of_key (eval_key: ejson -> option ejson) (k:ejson) (l: list ejson) :=
+    (lift_filter (fun d => ejson_key_is_eq_r eval_key d k) l).
+
+  Definition ejson_group_by_nested_eval (eval_key: ejson -> option ejson) (l: list ejson) : option (list (ejson * (list ejson))) :=
+    let dupkeys := lift_map (fun d => eval_key d) l in
+    let keys := lift bdistinct dupkeys in
+    olift (lift_map (fun k => olift (fun group => Some (k, group)) (ejson_group_of_key eval_key k l))) keys.
+
+  Definition ejson_group_to_partitions (g:string) (group: ejson * list ejson) : option ejson :=
+    match ejson_is_record (fst group) with
+    | Some keys =>
+      Some (ejobject (rec_concat_sort keys [(g, ejarray (snd group))]))
+    | _ => None
+    end.
+
+  Definition ejson_to_partitions (g:string) (l: list (ejson * list ejson)) :=
+    lift_map (ejson_group_to_partitions g) l.
+
+  Definition ejson_group_by_nested_eval_keys_partition
+             (g:string) (eval_keys:ejson -> option ejson) (l: list ejson) : option (list ejson) :=
+    olift (ejson_to_partitions g) (ejson_group_by_nested_eval eval_keys l).
+
+  Section tableform.
+    Definition ejson_group_by_nested_eval_table
+               (g:string) (sl:list string) (l:list ejson) : option (list ejson) :=
+      ejson_group_by_nested_eval_keys_partition
+        g
+        (fun j =>
+           match ejson_is_record j with
+           | Some r => Some (ejobject (rproject r sl))
+           | _ => None
+           end) l.
+
+  End tableform.
+
+End EJsonGroupBy.
+
