tests/sql/mini2.sql
@@ -1,0 +1,8 @@
+select
+	l_returnflag, count(*) as count
+from
+	lineitem
+where
+	l_shipdate <= date '1993-12-01'
+group by
+	l_returnflag;
